embedding/theories/pcuic/PCUICtoTemplate.v
@@ -3,6 +3,7 @@ From Coq Require Import Bool String List Program BinPos Compare_dec Omega.
 From MetaCoq.Template Require Import All.
      (* config utils AstUtils BasicAst Ast. *)
 From MetaCoq.PCUIC Require Import PCUICAst PCUICAstUtils PCUICInduction PCUICLiftSubst PCUICUnivSubst PCUICTyping PCUICGeneration.
+From MetaCoq.PCUIC Require Export PCUICToTemplate.
 Require Import String.
 Local Open Scope string_scope.
 Set Asymmetric Patterns.
@@ -10,45 +11,9 @@ Set Asymmetric Patterns.
 Module TC := Ast.
 Module P := PCUICAst.
 
-Fixpoint trans (t : P.term) : TC.term :=
-  match t with
-  | P.tRel n => TC.tRel n
-  | P.tVar n => TC.tVar n
-  | P.tEvar ev args => TC.tEvar ev (List.map trans args)
-  | P.tSort u => TC.tSort u
-  | P.tConst c u => TC.tConst c u
-  | P.tInd c u => TC.tInd c u
-  | P.tConstruct c k u => TC.tConstruct c k u
-  | P.tLambda na T M => TC.tLambda na (trans T) (trans M)
-  | P.tApp u v => TC.mkApps (trans u) [trans v]
-  | P.tProd na A B => TC.tProd na (trans A) (trans B)
-  | P.tLetIn na b t b' => TC.tLetIn na (trans b) (trans t) (trans b')
-  | P.tCase ind p c brs =>
-    let brs' := List.map (on_snd trans) brs in
-    TC.tCase ind (trans p) (trans c) brs'
-  | P.tProj p c => TC.tProj p (trans c)
-  | P.tFix mfix idx =>
-    let mfix' := List.map (map_def trans trans) mfix in
-    TC.tFix mfix' idx
-  | P.tCoFix mfix idx =>
-    let mfix' := List.map (map_def trans trans) mfix in
-    TC.tCoFix mfix' idx
-  end.
-
-Definition trans_decl (d : P.context_decl) :=
-  let 'P.mkdecl na b t := d in
-  {| TC.decl_name := na;
-     TC.decl_body := option_map trans b;
-     TC.decl_type := trans t |}.
-
-Definition trans_local Γ := List.map trans_decl Γ.
-
-Definition trans_one_ind_body (d : P.one_inductive_body) :=
-  {| TC.ind_name := d.(P.ind_name);
-     TC.ind_type := trans d.(P.ind_type);
-     TC.ind_kelim := d.(P.ind_kelim);
-     TC.ind_ctors := List.map (fun '(x, y, z) => (x, trans y, z)) d.(P.ind_ctors);
-     TC.ind_projs := List.map (fun '(x, y) => (x, trans y)) d.(P.ind_projs) |}.
+Definition aRelevant (n : name) : aname :=
+  {| binder_name := n;
+     binder_relevance := Relevant |}.
 
 Definition trans_local_entry (nle : ident * P.local_entry) : TC.context_decl :=
   let (nm, le) := nle in
@@ -58,9 +23,9 @@ Definition trans_local_entry (nle : ident * P.local_entry) : TC.context_decl :=
        bodies as parameters, so we produce a dummy value here.
        To produce an actual decalaration with a body we need its type,
        and it's not available it this point*)
-    TC.mkdecl (nNamed nm) None (TC.tVar "not supported")
+    TC.mkdecl (aRelevant (nNamed nm)) None (TC.tVar "not supported")
   | P.LocalAssum la =>
-    TC.mkdecl (nNamed nm) None (trans la)
+    TC.mkdecl (aRelevant (nNamed nm)) None (trans la)
   end.
 
 Definition trans_one_ind_entry (d : P.one_inductive_entry) : TC.one_inductive_entry :=
@@ -84,28 +49,3 @@ Definition trans_minductive_entry (e : P.mutual_inductive_entry) :  TC.mutual_in
      TC.mind_entry_universes := trans_universes_decl e.(P.mind_entry_universes);
      TC.mind_entry_variance := None;
      TC.mind_entry_private := e.(P.mind_entry_private) |}.
-
-Definition trans_constant_body (bd : P.constant_body) : TC.constant_body :=
-  {| TC.cst_type := trans bd.(P.cst_type);
-     TC.cst_body := option_map trans bd.(P.cst_body);
-     TC.cst_universes := bd.(P.cst_universes) |}.
-
-Definition trans_minductive_body md :=
-  {| TC.ind_finite := md.(P.ind_finite);
-     TC.ind_npars := md.(P.ind_npars);
-     TC.ind_params := trans_local md.(P.ind_params);
-     TC.ind_bodies := map trans_one_ind_body md.(P.ind_bodies);
-     TC.ind_variance := md.(ind_variance);
-     TC.ind_universes := md.(P.ind_universes) |}.
-
-Definition trans_global_decl (d : P.global_decl) : TC.global_decl :=
-  match d with
-  | P.ConstantDecl bd => TC.ConstantDecl (trans_constant_body bd)
-  | P.InductiveDecl bd => TC.InductiveDecl (trans_minductive_body bd)
-  end.
-
-Definition trans_global_env (d : P.global_env) :=
-  List.map (on_snd trans_global_decl) d.
-
-Definition trans_global (Σ : P.global_env_ext) : TC.global_env_ext :=
-  (trans_global_env (fst Σ), snd Σ).
